cp

ulib/FStar.Monotonic.Heap.fst
@@ -3,14 +3,6 @@ module FStar.Monotonic.Heap
 open FStar.Preorder
 open FStar.Classical
 
-(*
- * AR: we need to keep the preorder also in the heap
- * the reason is that, if we have two references of type a and same addr, say r1 and r2, and both are contained in a heap h
- * then we would like to enforce that their preorders are the same
- * otherwise, when updating one, we won't be able to prove that the second one also evolves per its preorder
- * by keeping preorder in the heap, we will ensure in the defn of contains that preorder also matches
- * moreover it's an option, for strongly typed refs (that are weakly contained in the heap), this woule be None
- *)
 private noeq type heap_rec = {
   next_addr: nat;
   memory   : nat -> Tot (option (a:Type0 & rel:(option (preorder a)) & a))
@@ -42,12 +34,6 @@ let contains #a #rel h r =
   Some? (h.memory r.addr) /\
   (let Some (| a1, pre_opt, _ |) = h.memory r.addr in
    a == a1 /\ Some? pre_opt /\ Some?.v pre_opt === rel)  //using `===` here, since otherwise typechecker fails with a and a1 being different types, why?
-
-let weak_contains h n =
-  let _ = () in
-  Some? (h.memory n) /\
-  (let Some (| _, pre_opt, _ |) = h.memory n in
-   None? pre_opt)
 
 let unused_in #a #rel r h = None? (h.memory r.addr)
 
@@ -97,8 +83,7 @@ private let lemma_upd_contains_test
 	   (forall (b:Type) (rel:preorder b) (r':ref b rel). (h0 `contains` r' /\ addr_of r' = addr_of r) ==> sel h1 r' == x /\
            (forall (b:Type) (rel:preorder b) (r':ref b rel). addr_of r' <> addr_of r ==> sel h0 r' == sel h1 r')             /\
 	   (forall (b:Type) (rel:preorder b) (r':ref b rel). h0 `contains` r' <==> h1 `contains` r')                         /\
-	   (forall (b:Type) (rel:preorder b) (r':ref b rel). r' `unused_in` h0  <==> r' `unused_in` h1)                      /\
-	   (forall (n:nat). h0 `weak_contains` n <==> h1 `weak_contains` n))))
+	   (forall (b:Type) (rel:preorder b) (r':ref b rel). r' `unused_in` h0  <==> r' `unused_in` h1))))
   = ()
 
 (*
@@ -128,8 +113,7 @@ private let lemma_upd_unused_test
 	   h1 `contains` r /\
            (forall (b:Type) (rel:preorder b) (r':ref b rel). addr_of r' <> addr_of r ==> sel h0 r' == sel h1 r') /\
 	   (forall (b:Type) (rel:preorder b) (r':ref b rel). h0 `contains` r' ==> h1 `contains` r')             /\
-	   (forall (b:Type) (rel:preorder b) (r':ref b rel). ~ (r' `unused_in` h0) ==> ~ (r' `unused_in` h1))   /\
-	   (forall (n:nat). h0 `weak_contains` n <==> h1 `weak_contains` n)))
+	   (forall (b:Type) (rel:preorder b) (r':ref b rel). ~ (r' `unused_in` h0) ==> ~ (r' `unused_in` h1))))
   = ()
 
 (*
@@ -151,8 +135,7 @@ private let lemma_free_mm_test (#a:Type) (rel:preorder a) (h0:heap) (r:ref a rel
 	  (forall (b:Type) (rel:preorder b) (r':ref b rel). addr_of r' <> addr_of r ==>
 	                          ((sel h0 r' == sel h1 r'                 /\
 				   (h0 `contains` r' <==> h1 `contains` r') /\
-				   (r' `unused_in` h0 <==> r' `unused_in` h1)))) /\
-	  (forall (n:nat). h0 `weak_contains` n <==> h1 `weak_contains` n))
+				   (r' `unused_in` h0 <==> r' `unused_in` h1)))))
   = ()
 
 private let lemma_alloc_fresh_test (#a:Type) (rel:preorder a) (h0:heap) (x:a) (mm:bool)
@@ -161,8 +144,12 @@ private let lemma_alloc_fresh_test (#a:Type) (rel:preorder a) (h0:heap) (x:a) (m
   = ()
 
 let lemma_contains_implies_used #a #rel h r = ()
+let lemma_contains_implies_not_weak_contains #a #rel h r = ()
+let lemma_weak_contains_implies_used #a #rel h r = ()
 let lemma_distinct_addrs_distinct_types #a #b #rel1 #rel2 h r1 r2 = ()
+let lemma_distinct_addrs_distinct_preorders #a #rel1 #rel2 h r1 r2 = ()
 let lemma_distinct_addrs_unused #a #b #rel1 #rel2 h r1 r2 = ()
+let lemma_distinct_addrs_weak_contains #a #b #rel1 #rel2 h r1 r2 = ()
 let lemma_alloc #a rel h0 x mm = ()
 let lemma_free_mm_sel #a #b #rel1 #rel2 h0 r1 r2 = ()
 let lemma_free_mm_contains #a #b #rel1 #rel2 h0 r1 r2 = ()
